---
tags:
  - "#review"
  - "#MATH117"
---
*Key Concepts:*
___

- The generalized conic section is defined as ==$Ax^2 + Bxy + Cy^2 + Dx + Ey + F = 0$==
	- ![[fzszgf7gquwjpzlbdzja1.jpg]]

- Note: With circles, the definition is
	- $\frac{(x-h)^2}{a^2} + \frac{(y - k)^2}{a^2} = 1$
	- $(x-h)^2 + (y - k)^2 = a^2$
	- $(x-h)^2 + (y - k)^2 = a^2$
	- Since h, k, and a are constants, this is essentially saying that: ==No matter what values of x and y you give, as long as they are on the circle, they will evaluate to a==

- Ellipses are defined as ==$\frac{(x-h)^2}{a^2}+\frac{(y-k)^2}{b^2}=1$==, where ==$(h, k)$== is the center of the ellipse, ==$a$== is the horizontal width of the ellipse, and ==$b$== is the vertical width of the ellipse. 
	- #TODO: Create an intuitive explanation for this / a proof, instead of just memorizing the above.
	- In the most simplified case, an ellipse can be conceptualized as the ==square root of a parabola that opens down. Since a square root has both positive and negative solutions, the parabola becomes a closed loop.==
	- When simplifying from general CS form to ellipse, make you need to realize that the quadratic terms are ==perfect squares==. 
		- This means that you need to ==complete the square== such that it is in the form $(x-h)^2$ and $(y-k)^2$
- To determine the form of a Conic Section (CS)
	- If ==$B^2 - 4AC < 0$==, it is either ==circle or ellipse.==
		- If ==$A = B$==, it is a ==circle==
		- if ==$A \ne B$==, it is an ==ellipse==. (Height and width)
	- If ==$B^2 - 4AC = 0$==, the CS is a ==parabola==
	- If ==$B^2-4AC > 0$== The CS is a ==hyperbola==
- The proof of using the determinant to evaluate the form of the CS:
	- ![[Pasted image 20251019134454.png|500]]
	- This equation looks like this: 
		- Aw hell nah I have no clue why this is true :( 
		- #TODO Ill have to ask my prof to explain, then make conceptual flashcards to repetitively prove it to yourself / explain it.
	- Just know that the sign of the ==quadratic y term== determines the form of the conic section, and that that is determined by ==$B^2 - 4AC$. 

- Def'n of Hyperbolas:
	- Hyperbolas have the same form as ellipses and circles, but its a ==difference instead of a sum==
		- Two possible forms:
			- ==$\frac{(x-h)^2}{a^2}-\frac{(y-k)^2}{b^2}=1$==: The branches open ==along the x axis==
				- The vertices are at ==$(h \pm a, k)$==
			- ==$\frac{(y-k)^2}{b^2}-\frac{(x-h)^2}{a^2} = 1$==: The branches open ==along the y axis==
				- The vertices are at ==$(h, k\pm b)$==
		- For both:
			- The hyperbola is centered at ==(h, k)==
			- The equation for the asymptotes are ==$y = \pm \frac{a}{b}(x-h)+k$
			- the denom a corresponds to the ==x== term, and the denom b corresponds to the ==y== term.
*Terms and Definitions:
___ <!--SR:!2025-10-20,1,230!2000-01-01,1,250!2000-01-01,1,250!2000-01-01,1,250!2000-01-01,1,250!2000-01-01,1,250!2000-01-01,1,250!2000-01-01,1,250!2000-01-01,1,250!2000-01-01,1,250-->


*Common Mistakes:*
___
