---
tags:
  - "#review"
  - "#flashcards"
sr-due: 2025-09-20
sr-interval: 3
sr-ease: 250
---
*Key Concepts:*
___

- We can use chain rule to derive the Inverse Function Theorem (IFT):
	- We are given that $f(f^-1(x)) = x$
	- $\frac{\mathrm{d}}{\mathrm{dx}}(f(f^{-1}(x))) = \frac{\mathrm{d}}{\mathrm{dx}}x$
	- $\frac{\mathrm{d}}{\mathrm{dx}}f(f^{-1}(x))\cdot \frac{\mathrm{d}}{\mathrm{dx}}(f^{-1}(x)) = 1$
	- $\frac{\mathrm{d}}{\mathrm{dx}}f^{-1}(x) = \frac{1}{\frac{\mathrm{d}}{\mathrm{dx}}f(f^{-1}(x))}$

- In other words ==you can use knowledge of the inverse of f(x)s to find the derivative of the inverse of x==

*Examples (Excluding inline examples)* 
___

*Significant Theorems:*
___

*Respective Proofs*
___

*Common Mistakes:*
___

*Terms and Definitions:*
___

